\documentclass{article}
\usepackage{amsmath}

\begin{document}
\title{Maths Assignment}
\author{Karyampudi Meghana Sai\\
        EE23BTECH11031}
\maketitle
\section*{Problem Statement}

The ratio of the A.M and G.M of two positive numbers $a$ and $b$ is $m:n$. Show that $a:b = \left( m + \sqrt{m^2 - n^2} \right) : \left( m - \sqrt{m^2 - n^2} \right)$.
\section*{Solution}

Expressing A.M and G.M in terms of $a$ and $b$:
\[ \frac{a + b}{2\sqrt{ab}} = \frac{m}{n} \]

From the given expression, let's express $a$ and $b$ in terms of $m$ and $n$ using the quadratic equation.


Let's assume that $x = \sqrt{\frac{a}{b}}$. Then, we have:
\[ \frac{a}{b} = x^2 \]

Substituting this into the equation for A.M and G.M:
\[ \frac{1 + x^2}{2x} = \frac{m}{n} \]
\[ \frac{1}{x} + x = \frac{2m}{n} \]
\[ x^2 - \frac{2m}{n}x + 1 = 0 \]

This is a quadratic equation in terms of $x$, and the roots of this equation are $x = \frac{2m}{n} \pm \sqrt{\left(\frac{2m}{n}\right)^2 - 4}$. Simplifying the expression inside the square root gives us:

\[ x = \frac{2m}{n} \pm \sqrt{\frac{4m^2}{n^2} - 4} \]
\[ x = \frac{2m}{n} \pm \sqrt{\frac{4m^2 - 4n^2}{n^2}} \]
\[ x = \frac{2m}{n} \pm \frac{2}{n} \sqrt{m^2 - n^2} \]

Since $x = \sqrt{\frac{a}{b}}$, $x$ must be positive, so we take the positive sign before the square root. Therefore:
\[ x = \frac{2m}{n} + \frac{2}{n} \sqrt{m^2 - n^2} \]
\[ x = \frac{2}{n}(m + \sqrt{m^2 - n^2}) \]

Now, since $x = \sqrt{\frac{a}{b}}$, we have:
\[ \frac{a}{b} = \left(\frac{2}{n}\right)^2 (m + \sqrt{m^2 - n^2})^2 \]

Now, let's express $a:b$ using this result:
\[ \frac{a}{b} = \frac{4}{n^2}(m + \sqrt{m^2 - n^2})^2 \]
Multiplying both the numerator and denominator with ($m-\sqrt{m^2 - n^2}$): 
\[ \frac{a}{b} = \frac{4}{n^2} \frac{(m + \sqrt{m^2 - n^2})^2  (m-\sqrt{m^2 - n^2})}{(m-\sqrt{m^2 - n^2})}\]

\[ a:b = 2 \left( m + \sqrt{m^2 - n^2} \right) : 2 \left( m - \sqrt{m^2 - n^2} \right) \]

Finally, simplify by dividing both sides by 2:
\[ a:b = \left( m + \sqrt{m^2 - n^2} \right) : \left( m - \sqrt{m^2 - n^2} \right) \]

Thus, we've arrived at the required result: $a:b = \left( m + \sqrt{m^2 - n^2} \right) : \left( m - \sqrt{m^2 - n^2} \right)$.

\end{document}

